tests/Schedule.bpl
@@ -1,15 +1,19 @@
-
 // ---------------------------------------------------------------
 // -- Types and global variables ---------------------------------
 // ---------------------------------------------------------------
 type Chan a;
+type Actor;
 type CType = <a>[Chan a]int;
 type MType = <a>[Chan a][int]a;
 type State;
+
 var M: MType;
 var C: CType;
 var R: CType; 
 var C#init: CType;
+var St: [Actor]State;
+
+const unique this#: Actor;
 
 // ---------------------------------------------------------------
 // -- End of prelude ---------------------------------------------
@@ -18,38 +22,42 @@ var C#init: CType;
 const unique FairMerge#s1: State;
 const unique FairMerge#s2: State;
 procedure FairMerge#a1()
+  modifies C, R, M, St;
 {
-  var A#State: State;
+  var this#: Actor;
   var i: int;
-  assume (A#State == FairMerge#s1) || (A#State == FairMerge#s2);
-  assume A#State == FairMerge#s1;
+  assume (St[this#] == FairMerge#s1) || (St[this#] == FairMerge#s2);
+  assume St[this#] == FairMerge#s1;
   assume true;
-  A#State := FairMerge#s2;
-  assert {:msg "  1.1: Action might not preserve invariant"} (A#State == FairMerge#s1) || (A#State == FairMerge#s2);
+  St[this#] := FairMerge#s2;
+  assert {:msg "  1.1: Action might not preserve invariant"} (St[this#] == FairMerge#s1) || (St[this#] == FairMerge#s2);
 }
 procedure FairMerge#a2()
+  modifies C, R, M, St;
 {
-  var A#State: State;
+  var this#: Actor;
   var i: int;
-  assume (A#State == FairMerge#s1) || (A#State == FairMerge#s2);
-  assume A#State == FairMerge#s2;
+  assume (St[this#] == FairMerge#s1) || (St[this#] == FairMerge#s2);
+  assume St[this#] == FairMerge#s2;
   assume true;
-  A#State := FairMerge#s1;
-  assert {:msg "  1.1: Action might not preserve invariant"} (A#State == FairMerge#s1) || (A#State == FairMerge#s2);
+  St[this#] := FairMerge#s1;
+  assert {:msg "  1.1: Action might not preserve invariant"} (St[this#] == FairMerge#s1) || (St[this#] == FairMerge#s2);
 }
+const unique Top#fm: Actor;
 const unique Top#a: Chan (int);
 const unique Top#b: Chan (int);
 const unique Top#c: Chan (int);
 procedure Top#anon$0#entry()
-  modifies C, R, M;
+  modifies C, R, M, St;
 {
-  assume C#init[Top#a] == 2;
-  assume C#init[Top#b] == 0;
+  assume C#init[Top#a] == 1;
+  assume C#init[Top#b] == 1;
   assume C#init[Top#c] == 0;
   assume R[Top#a] == 0;
   assume R[Top#b] == 0;
   assume R[Top#c] == 0;
   assume C#init == C;
+  assume St[Top#fm] == FairMerge#s1;
   assert {:msg "  Channel invariant might not hold on action entry"} R[Top#c] == 0;
   assert {:msg "  Channel invariant might not hold on action entry"} 0 <= C[Top#c];
   assert {:msg "  Channel invariant might not hold on action entry"} 0 <= R[Top#c];
@@ -59,14 +67,22 @@ procedure Top#anon$0#entry()
   assert {:msg "  Channel invariant might not hold on action entry"} (R[Top#a] + C[Top#a]) == C#init[Top#a];
   assert {:msg "  Channel invariant might not hold on action entry"} 0 <= C[Top#a];
   assert {:msg "  Channel invariant might not hold on action entry"} 0 <= R[Top#a];
-  assert {:msg "  14.15: Channel invariant might not hold on action entry"} (R[Top#c] + C[Top#c]) == (R[Top#a] + R[Top#b]);
+  assert {:msg "  16.15: Channel invariant might not hold on action entry"} (R[Top#c] + C[Top#c]) == (R[Top#a] + R[Top#b]);
+  assert {:msg "  17.15: Channel invariant might not hold on action entry"} ((R[Top#c] + C[Top#c]) >= 1) ==> (C[Top#a] == 0);
+  assert {:msg "  18.15: Channel invariant might not hold on action entry"} ((R[Top#c] + C[Top#c]) >= 2) ==> (C[Top#b] == 0);
+  assert {:msg "  19.15: Channel invariant might not hold on action entry"} (R[Top#a] == 0) && (R[Top#b] == 0) ==> (St[Top#fm] == FairMerge#s1);
+  assert {:msg "  20.15: Channel invariant might not hold on action entry"} (R[Top#a] == 1) && (R[Top#b] == 0) ==> (St[Top#fm] == FairMerge#s2);
+  assert {:msg "  21.15: Channel invariant might not hold on action entry"} (R[Top#a] == 1) && (R[Top#b] == 1) ==> (St[Top#fm] == FairMerge#s1);
+  assert {:msg "  23.15: Channel invariant might not hold on action entry"} ((R[Top#c] + C[Top#c]) >= 1) ==> (M[Top#c][0] == M[Top#a][0]);
+  assert {:msg "  24.15: Channel invariant might not hold on action entry"} ((R[Top#c] + C[Top#c]) >= 2) ==> (M[Top#c][1] == M[Top#b][0]);
 }
 procedure Top#anon$0#FairMerge#a1()
-  modifies C, R, M;
+  modifies C, R, M, St;
 {
+  var St#next: State;
   var x1#i: int;
-  assume C#init[Top#a] == 2;
-  assume C#init[Top#b] == 0;
+  assume C#init[Top#a] == 1;
+  assume C#init[Top#b] == 1;
   assume C#init[Top#c] == 0;
   assume R[Top#c] == 0;
   assume 0 <= C[Top#c];
@@ -78,12 +94,22 @@ procedure Top#anon$0#FairMerge#a1()
   assume 0 <= C[Top#a];
   assume 0 <= R[Top#a];
   assume (R[Top#c] + C[Top#c]) == (R[Top#a] + R[Top#b]);
-  assume 1 <= C[Top#a];
+  assume ((R[Top#c] + C[Top#c]) >= 1) ==> (C[Top#a] == 0);
+  assume ((R[Top#c] + C[Top#c]) >= 2) ==> (C[Top#b] == 0);
+  assume (R[Top#a] == 0) && (R[Top#b] == 0) ==> (St[Top#fm] == FairMerge#s1);
+  assume (R[Top#a] == 1) && (R[Top#b] == 0) ==> (St[Top#fm] == FairMerge#s2);
+  assume (R[Top#a] == 1) && (R[Top#b] == 1) ==> (St[Top#fm] == FairMerge#s1);
+  assume ((R[Top#c] + C[Top#c]) >= 1) ==> (M[Top#c][0] == M[Top#a][0]);
+  assume ((R[Top#c] + C[Top#c]) >= 2) ==> (M[Top#c][1] == M[Top#b][0]);
+  assume St[Top#fm] == FairMerge#s1;
+  assume (1 <= C[Top#a]) && (St[Top#fm] == FairMerge#s1);
   x1#i := M[Top#a][R[Top#a]];
   R[Top#a] := R[Top#a] + 1;
   C[Top#a] := C[Top#a] - 1;
   M[Top#c][R[Top#c] + C[Top#c]] := x1#i;
   C[Top#c] := C[Top#c] + 1;
+  assume St#next == FairMerge#s2;
+  St[Top#fm] := St#next;
   assert {:msg "  Sub-actor action at 2.3 might not preserve the channel invariant"} R[Top#c] == 0;
   assert {:msg "  Sub-actor action at 2.3 might not preserve the channel invariant"} 0 <= C[Top#c];
   assert {:msg "  Sub-actor action at 2.3 might not preserve the channel invariant"} 0 <= R[Top#c];
@@ -93,14 +119,22 @@ procedure Top#anon$0#FairMerge#a1()
   assert {:msg "  Sub-actor action at 2.3 might not preserve the channel invariant"} (R[Top#a] + C[Top#a]) == C#init[Top#a];
   assert {:msg "  Sub-actor action at 2.3 might not preserve the channel invariant"} 0 <= C[Top#a];
   assert {:msg "  Sub-actor action at 2.3 might not preserve the channel invariant"} 0 <= R[Top#a];
-  assert {:msg "  14.15: Sub-actor action at 2.3 might not preserve the channel invariant"} (R[Top#c] + C[Top#c]) == (R[Top#a] + R[Top#b]);
+  assert {:msg "  16.15: Sub-actor action at 2.3 might not preserve the channel invariant"} (R[Top#c] + C[Top#c]) == (R[Top#a] + R[Top#b]);
+  assert {:msg "  17.15: Sub-actor action at 2.3 might not preserve the channel invariant"} ((R[Top#c] + C[Top#c]) >= 1) ==> (C[Top#a] == 0);
+  assert {:msg "  18.15: Sub-actor action at 2.3 might not preserve the channel invariant"} ((R[Top#c] + C[Top#c]) >= 2) ==> (C[Top#b] == 0);
+  assert {:msg "  19.15: Sub-actor action at 2.3 might not preserve the channel invariant"} (R[Top#a] == 0) && (R[Top#b] == 0) ==> (St[Top#fm] == FairMerge#s1);
+  assert {:msg "  20.15: Sub-actor action at 2.3 might not preserve the channel invariant"} (R[Top#a] == 1) && (R[Top#b] == 0) ==> (St[Top#fm] == FairMerge#s2);
+  assert {:msg "  21.15: Sub-actor action at 2.3 might not preserve the channel invariant"} (R[Top#a] == 1) && (R[Top#b] == 1) ==> (St[Top#fm] == FairMerge#s1);
+  assert {:msg "  23.15: Sub-actor action at 2.3 might not preserve the channel invariant"} ((R[Top#c] + C[Top#c]) >= 1) ==> (M[Top#c][0] == M[Top#a][0]);
+  assert {:msg "  24.15: Sub-actor action at 2.3 might not preserve the channel invariant"} ((R[Top#c] + C[Top#c]) >= 2) ==> (M[Top#c][1] == M[Top#b][0]);
 }
 procedure Top#anon$0#FairMerge#a2()
-  modifies C, R, M;
+  modifies C, R, M, St;
 {
+  var St#next: State;
   var x2#i: int;
-  assume C#init[Top#a] == 2;
-  assume C#init[Top#b] == 0;
+  assume C#init[Top#a] == 1;
+  assume C#init[Top#b] == 1;
   assume C#init[Top#c] == 0;
   assume R[Top#c] == 0;
   assume 0 <= C[Top#c];
@@ -112,12 +146,22 @@ procedure Top#anon$0#FairMerge#a2()
   assume 0 <= C[Top#a];
   assume 0 <= R[Top#a];
   assume (R[Top#c] + C[Top#c]) == (R[Top#a] + R[Top#b]);
-  assume 1 <= C[Top#b];
+  assume ((R[Top#c] + C[Top#c]) >= 1) ==> (C[Top#a] == 0);
+  assume ((R[Top#c] + C[Top#c]) >= 2) ==> (C[Top#b] == 0);
+  assume (R[Top#a] == 0) && (R[Top#b] == 0) ==> (St[Top#fm] == FairMerge#s1);
+  assume (R[Top#a] == 1) && (R[Top#b] == 0) ==> (St[Top#fm] == FairMerge#s2);
+  assume (R[Top#a] == 1) && (R[Top#b] == 1) ==> (St[Top#fm] == FairMerge#s1);
+  assume ((R[Top#c] + C[Top#c]) >= 1) ==> (M[Top#c][0] == M[Top#a][0]);
+  assume ((R[Top#c] + C[Top#c]) >= 2) ==> (M[Top#c][1] == M[Top#b][0]);
+  assume St[Top#fm] == FairMerge#s2;
+  assume (1 <= C[Top#b]) && (St[Top#fm] == FairMerge#s2);
   x2#i := M[Top#b][R[Top#b]];
   R[Top#b] := R[Top#b] + 1;
   C[Top#b] := C[Top#b] - 1;
   M[Top#c][R[Top#c] + C[Top#c]] := x2#i;
   C[Top#c] := C[Top#c] + 1;
+  assume St#next == FairMerge#s1;
+  St[Top#fm] := St#next;
   assert {:msg "  Sub-actor action at 3.3 might not preserve the channel invariant"} R[Top#c] == 0;
   assert {:msg "  Sub-actor action at 3.3 might not preserve the channel invariant"} 0 <= C[Top#c];
   assert {:msg "  Sub-actor action at 3.3 might not preserve the channel invariant"} 0 <= R[Top#c];
@@ -127,13 +171,20 @@ procedure Top#anon$0#FairMerge#a2()
   assert {:msg "  Sub-actor action at 3.3 might not preserve the channel invariant"} (R[Top#a] + C[Top#a]) == C#init[Top#a];
   assert {:msg "  Sub-actor action at 3.3 might not preserve the channel invariant"} 0 <= C[Top#a];
   assert {:msg "  Sub-actor action at 3.3 might not preserve the channel invariant"} 0 <= R[Top#a];
-  assert {:msg "  14.15: Sub-actor action at 3.3 might not preserve the channel invariant"} (R[Top#c] + C[Top#c]) == (R[Top#a] + R[Top#b]);
+  assert {:msg "  16.15: Sub-actor action at 3.3 might not preserve the channel invariant"} (R[Top#c] + C[Top#c]) == (R[Top#a] + R[Top#b]);
+  assert {:msg "  17.15: Sub-actor action at 3.3 might not preserve the channel invariant"} ((R[Top#c] + C[Top#c]) >= 1) ==> (C[Top#a] == 0);
+  assert {:msg "  18.15: Sub-actor action at 3.3 might not preserve the channel invariant"} ((R[Top#c] + C[Top#c]) >= 2) ==> (C[Top#b] == 0);
+  assert {:msg "  19.15: Sub-actor action at 3.3 might not preserve the channel invariant"} (R[Top#a] == 0) && (R[Top#b] == 0) ==> (St[Top#fm] == FairMerge#s1);
+  assert {:msg "  20.15: Sub-actor action at 3.3 might not preserve the channel invariant"} (R[Top#a] == 1) && (R[Top#b] == 0) ==> (St[Top#fm] == FairMerge#s2);
+  assert {:msg "  21.15: Sub-actor action at 3.3 might not preserve the channel invariant"} (R[Top#a] == 1) && (R[Top#b] == 1) ==> (St[Top#fm] == FairMerge#s1);
+  assert {:msg "  23.15: Sub-actor action at 3.3 might not preserve the channel invariant"} ((R[Top#c] + C[Top#c]) >= 1) ==> (M[Top#c][0] == M[Top#a][0]);
+  assert {:msg "  24.15: Sub-actor action at 3.3 might not preserve the channel invariant"} ((R[Top#c] + C[Top#c]) >= 2) ==> (M[Top#c][1] == M[Top#b][0]);
 }
 procedure Top#anon$0#exit()
-  modifies C, R, M;
+  modifies C, R, M, St;
 {
-  assume C#init[Top#a] == 2;
-  assume C#init[Top#b] == 0;
+  assume C#init[Top#a] == 1;
+  assume C#init[Top#b] == 1;
   assume C#init[Top#c] == 0;
   assume R[Top#c] == 0;
   assume 0 <= C[Top#c];
@@ -145,12 +196,20 @@ procedure Top#anon$0#exit()
   assume 0 <= C[Top#a];
   assume 0 <= R[Top#a];
   assume (R[Top#c] + C[Top#c]) == (R[Top#a] + R[Top#b]);
-  assume !((1 <= C[Top#a]) || (1 <= C[Top#b]));
+  assume ((R[Top#c] + C[Top#c]) >= 1) ==> (C[Top#a] == 0);
+  assume ((R[Top#c] + C[Top#c]) >= 2) ==> (C[Top#b] == 0);
+  assume (R[Top#a] == 0) && (R[Top#b] == 0) ==> (St[Top#fm] == FairMerge#s1);
+  assume (R[Top#a] == 1) && (R[Top#b] == 0) ==> (St[Top#fm] == FairMerge#s2);
+  assume (R[Top#a] == 1) && (R[Top#b] == 1) ==> (St[Top#fm] == FairMerge#s1);
+  assume ((R[Top#c] + C[Top#c]) >= 1) ==> (M[Top#c][0] == M[Top#a][0]);
+  assume ((R[Top#c] + C[Top#c]) >= 2) ==> (M[Top#c][1] == M[Top#b][0]);
+  assume !(((1 <= C[Top#a]) && (St[Top#fm] == FairMerge#s1)) || ((1 <= C[Top#b]) && (St[Top#fm] == FairMerge#s2)));
   assert {:msg "  12.3: The network might leave unread tokens on channel a"} C[Top#a] == 0;
   assert {:msg "  12.3: The network might leave unread tokens on channel b"} C[Top#b] == 0;
   assert {:msg "  12.3: The network might not produce the specified number of tokens on output out"} C[Top#c] == 2;
-  assert {:msg "  12.29: Network output might not conform to specified action output"} M[Top#c][0] == M[Top#a][0];
-  assert {:msg "  12.31: Network output might not conform to specified action output"} M[Top#c][1] == M[Top#a][1];
+  assert {:msg "  12.36: Network output might not conform to specified action output"} M[Top#c][0] == M[Top#a][0];
+  assert {:msg "  12.38: Network output might not conform to specified action output"} M[Top#c][1] == M[Top#b][0];
   R[Top#c] := R[Top#c] + C[Top#c];
   C[Top#c] := 0;
+  assert {:msg "  14.13: The network might not preserve the network invariant"} St[Top#fm] == FairMerge#s1;
 }
